\begin{answer}

$$
p(y=1\mid x;\phi,\mu_0,\mu_1,\Sigma)
= \frac{p(x\mid y=1)p(y=1)}
       {p(x\mid y=1)p(y=1) + p(x\mid y=0)p(y=0)}
$$
Rewrite the posterior following $\frac{a}{a+b} = \frac{1}{a^{-1}} \frac{1}{a+b} = \frac{1}{1+a^{-1}b}$
$$
p(y=1\mid x;\phi,\mu_0,\mu_1,\Sigma)
= \frac{1}
       {1 + \frac{p(x\mid y=0)p(y=0)}{p(x\mid y=1)p(y=1)}}
$$
Then, to comply with the logistics form:
$$
p(y=1\mid x;\phi,\mu_0,\mu_1,\Sigma)
= \frac{1}
       {1 + \exp \log \left( \frac{p(x\mid y=0)p(y=0)}{p(x\mid y=1)p(y=1)} \right)}
$$
$$
\log\frac{p(x\mid y=0)p(y=0)}{p(x\mid y=1)p(y=1)}
= \log \frac{p(x\mid y=0)}{p(x\mid y=1)}
+ \log \frac{p(y=0)}{p(y=1)}
$$
And
$$
p(x\mid y=i)
= \frac{1}{(2\pi)^{d/2}|\Sigma|^{1/2}}
  \exp\!\left(-\frac12(x-\mu_i)^{\top}\Sigma^{-1}(x-\mu_i)\right),
  \quad i\in\{0,1\}.
$$
So
$$
\begin{align}
\log \frac{p(x\mid y=0)}{p(x\mid y=1)}
&= -\frac{1}{2}\Big[
(x-\mu_0)^{\top}\Sigma^{-1}(x-\mu_0)
- (x-\mu_1)^{\top}\Sigma^{-1}(x-\mu_1)
\Big] \\
&= x^{\top}\Sigma^{-1}(\mu_0-\mu_1)
   + \tfrac{1}{2}(\mu_1^{\top}\Sigma^{-1}\mu_1 - \mu_0^{\top}\Sigma^{-1}\mu_0)
\end{align}
$$
$$
\log \frac{p(y=0)}{p(y=1)} = \log \frac{1-\phi}{\phi} = - \log \frac{\phi}{1-\phi}
$$
$$
\exp \log \left( \frac{p(x\mid y=0)p(y=0)}{p(x\mid y=1)p(y=1)} \right)
= \exp \left(
(\mu_0-\mu_1)^{\top}\Sigma^{-1}x
   + \tfrac{1}{2}(\mu_1^{\top}\Sigma^{-1}\mu_1 - \mu_0^{\top}\Sigma^{-1}\mu_0)
+ \log \frac{1-\phi}{\phi}
\right)
$$
Then, the values of $\theta$ and $\theta_{0}$ to match the logistic form are:

$$
\boxed{
\theta = \Sigma^{-1}(\mu_{1}-\mu_{0})
}
$$
$$
\boxed{
\theta_{0} 
= \tfrac{1}{2}(\mu_0^{\top}\Sigma^{-1}\mu_0 - \mu_1^{\top}\Sigma^{-1}\mu_1)
+ \log \frac{\phi}{1-\phi}
}
$$
\end{answer}
