\begin{answer}

$$
\begin{aligned}
\ell(\theta)
&=\sum_{i=1}^n \log p(x^{(i)},y^{(i)};\theta)\\
&=\sum_{i=1}^n \log p(x^{(i)}\mid y^{(i)};\mu_0,\mu_1,\Sigma)+\sum_{i=1}^n \log p(y^{(i)};\phi)\\
&=\sum_{i=1}^n\Bigg[-\frac{d}{2}\log(2\pi)-\frac{1}{2}\log|\Sigma|
-\frac{1}{2}\big(x^{(i)}-\mu_{y^{(i)}}\big)^\top\Sigma^{-1}\big(x^{(i)}-\mu_{y^{(i)}}\big)\Bigg]\\
&\quad +\sum_{i=1}^n\Big[y^{(i)}\log\phi+\big(1-y^{(i)}\big)\log(1-\phi)\Big]
\end{aligned}
$$
Constants can be ignored when maximizing the log-likelihood, so we have
$$
\begin{aligned}
\ell(\theta)
&=-\frac{n}{2}\log|\Sigma| - \frac{1}{2}\sum_{i=1}^n\big(x^{(i)}-\mu_{
y^{(i)}}\big)^\top\Sigma^{-1}\big(x^{(i)}-\mu_{y^{(i)}}\big)\\
&\quad +\sum_{i=1}^n\Big[y^{(i)}\log\phi+\big(1-y^{(i)}\big)\log(1-\phi)\Big]
\end{aligned}
$$
For $\phi$, we have
$$
\begin{aligned}
\frac{\partial}{\partial \phi}\ell(\theta)
&=\sum_{i=1}^n\Big[\frac{y^{(i)}}{\phi}-\frac{1-y^{(i)}}{1-\phi}\Big]\\
&=\frac{1}{\phi(1-\phi)}\Big[\sum_{i=1}^n y^{(i)} - n\phi\Big]
\end{aligned}
$$
Setting this to zero,
$$
\boxed{
\phi = \frac{1}{n}\sum_{i=1}^n y^{(i)}
}
$$
For $\mu_0$, we care for those with $y^{(i)}=0$, so
$$
\ell(\mu_0) = -\frac{1}{2}\sum_{i=1}^n \mathbf{1}\{y^{(i)}=0\}
\big(x^{(i)}-\mu_0\big)^\top\Sigma^{-1}\big(x^{(i)}-\mu_0\big) + \text{const}
$$
$$
\begin{aligned}
\frac{\partial \ell}{\partial \mu_0}
&= -\frac{1}{2}\sum_{i=1}^n \mathbf{1}\{y^{(i)}=0\}\cdot 
\big(-2\Sigma^{-1}(x^{(i)}-\mu_0)\big)\\
&=\Sigma^{-1}\sum_{i=1}^n \mathbf{1}\{y^{(i)}=0\}\big(x^{(i)}-\mu_0\big)
\end{aligned}
$$
Setting this to zero,
$$
\sum_{i=1}^n \mathbf{1}\{y^{(i)}=0\}x^{(i)}=
\left(\sum_{i=1}^n \mathbf{1}\{y^{(i)}=0\}\right)\mu_0
\;\therefore\;
\boxed{\;\displaystyle \mu_0=\frac{\sum_{i=1}^n \mathbf{1}\{y^{(i)}=0\}x^{(i)}}{\sum_{i=1}^n \mathbf{1}\{y^{(i)}=0\}}\; }
$$
Similarly, for $\mu_1$, we have
$$
\boxed{\;\displaystyle \mu_1=\frac{\sum_{i=1}^n \mathbf{1}\{y^{(i)}=1\}x^{(i)}}{\sum_{i=1}^n \mathbf{1}\{y^{(i)}=1\}}\; }.
$$
For $\Sigma$, we have
$$
\ell(\Sigma)=-\frac{n}{2}\log|\Sigma|-\frac{1}{2}\sum_{i=1}^n
\big(x^{(i)}-\mu_{y^{(i)}}\big)^\top\Sigma^{-1}\big(x^{(i)}-\mu_{y^{(i)}}\big)+\text{const}
$$
The quadratic term can be rewritten as a trace, so
$$
\ell(\Sigma)=-\frac{n}{2}\log|\Sigma|-\frac{1}{2}\sum_{i=1}^n
\text{tr}(\Sigma^{-1}\big(x^{(i)}-\mu_{y^{(i)}}\big)\big(x^{(i)}-\mu_{y^{(i)}}\big)^\top)
$$
$$
\frac{\partial \ell}{\partial \Sigma}
=-\frac{n}{2}\Sigma^{-1}+\frac{1}{2}\sum_{i=1}^n\Sigma^{-1}\big(x^{(i)}-\mu_{y^{(i)}}\big)\big(x^{(i)}-\mu_{y^{(i)}}\big)^\top\Sigma^{-1}.
$$
Setting this to zero,
$$
\boxed{
\Sigma = \frac{1}{n}\sum_{i=1}^n \big(x^{(i)}-\mu_{y^{(i)}}\big)\big(x^{(i)}-\mu_{y^{(i)}}\big)^\top
}
$$
\end{answer}
