\begin{answer}

Let $\eta=\theta^\top x$. For one example $(x,y)$ with $y\in\{0,1\}$,
the (negative) log-likelihood (logistic loss) is
\[
\ell(\theta) \;=\; -\Big( y\log g(\eta) + (1-y)\log(1-g(\eta)) \Big).
\]

Gradient (w. chain-rule).
Differentiate w.r.t.\ $\eta$ first and then w.r.t. $\theta$:
\[
\frac{\partial \ell}{\partial \eta}
= -\Big( y\,\frac{1}{g(\eta)}\,\frac{\partial g(\eta)}{\partial \eta}
       + (1-y)\,\frac{1}{1-g(\eta)}\,\frac{\partial (1-g(\eta))}{\partial \eta} \Big)
= -\Big( y\,\frac{1}{g(\eta)}\,g(\eta)' \;-\; (1-y)\,\frac{1}{1-g(\eta)}\,g(\eta)' \Big),
\]
since $\dfrac{\partial (1-g(\eta))}{\partial \eta} = -g(\eta)'$. Using $g(\eta)'=\dfrac{\partial g(\eta)}{\partial \eta} = g(\eta)(1-g(\eta))$,
\[
\frac{\partial \ell}{\partial \eta}
= -\,y\,\frac{g(\eta)(1-g(\eta))}{g(\eta)} \;+\; (1-y)\,\frac{g(\eta)(1-g(\eta))}{1-g(\eta)}
= -(y(1-g(\eta))) \;+\; (1-y)g(\eta) 
= g(\eta) - y.
\]
Therefore,
\[
\nabla_\theta \ell(\theta)
= \frac{\partial \ell}{\partial \eta}\,\frac{\partial \eta}{\partial \theta}
= (g(\eta)-y)\,x.
\]

Hessian
\[
\nabla_\theta^2 \ell(\theta)
= \nabla_\theta\!\big((g(\eta)-y)\,x\big)
= \big(\nabla_\theta g(\eta)\big)\,x^\top
= \Big(\frac{\partial g(\eta)}{\partial \eta}\,\frac{\partial \eta}{\partial \theta}\Big)\,x^\top
= g'(\eta)\,x\,x^\top
= g(\eta)(1-g(\eta))\,x\,x^\top.
\]

Verification
For any $z\in\mathbb{R}^d$,
\[
z^\top \nabla_\theta^2 \ell(\theta)\, z
= z^\top (g(\eta)(1-g(\eta))\,x\,x^\top) z
= g(\eta)(1-g(\eta))\, (z^\top x)^2 \;\ge\; 0,
\]
because $g(\eta)(1-g(\eta))\ge 0$ and $(z^\top x)^2\ge 0$. Hence $\nabla_\theta^2 \ell(\theta)\succeq 0$.

%\paragraph{Dataset form (for completeness).}
%For $n$ examples $\{(x^{(i)},y^{(i)})\}_{i=1}^n$,
%\[
%J(\theta) \;=\; \frac{1}{n}\sum_{i=1}^n \ell^{(i)}(\theta),
%\qquad
%\nabla_\theta^2 J(\theta) \;=\; \frac{1}{n}\sum_{i=1}^n g(\eta)_i(1-g(\eta)_i)\,x^{(i)}{x^{(i)}}^\top,
%\]
%with $g(\eta)_i=g(\theta^\top x^{(i)})$. Thus for any $z$,
%\[
%z^\top \big(\nabla_\theta^2 J(\theta)\big) z
%= \frac{1}{n}\sum_{i=1}^n g(\eta)_i(1-g(\eta)_i)\,(z^\top x^{(i)})^2 \;\ge\; 0,
%\]
%so $\nabla_\theta^2 J(\theta)\succeq 0$.
% (Vectorized: with X having rows x^{(i)} and S=diag(h_i(1-h_i)), \; \nabla^2 J = \tfrac{1}{n} X^\top S X \succeq 0.)


\end{answer}
