\begin{answer}

Differentiate $\E[Y;\eta]=a'(\eta)$ w.r.t.\ $\eta$:
\[
\frac{d}{d\eta}a'(\eta)
    \;=\; \frac{d}{d\eta}\E[Y;\eta]
    \;=\; \int y \frac{d}{d\eta} \, p(y;\eta)
\]
\[
    \;=\; \int y\,(y - a'(\eta))\,p(y;\eta)\,dy
    \;=\; \int y^2\,p(y;\eta)\,dy - \int \,y\,a'(\eta)\,p(y;\eta)\,dy\,
\]
\[
   a''(\eta) \;=\; \E[Y^2;\eta] \,-\, a'(\eta)\E[Y;\eta]
\]

But $\E[Y;\eta]=a'(\eta)$, so
\[
   a''(\eta) \;=\; \E[Y^2;\eta] \,-\, \E[Y;\eta]^2 = \E[Y - \E[{Y;\eta];\eta}]^2
\]
\[
\boxed{\,\text{Var}(Y;\eta) \;=\; a''(\eta)\,}
\]

\end{answer}
