\begin{answer}

Let the activations be defined as:
$$
a^{(i)}_2 = w^{[1]}_{0,2} + w^{[1]}_{1,2}x^{(i)}_1 + w^{[1]}_{2,2}x^{(i)}_2,
\quad
h^{(i)}_2 = \sigma(a^{(i)}_2),
$$
$$
z^{(i)} = w^{[2]}_0 + \sum_{j=1}^{3} w^{[2]}_j h^{(i)}_j,
\quad
o^{(i)} = \sigma(z^{(i)}),
$$
where $\sigma(u)=\frac{1}{1+e^{-u}}$.

The loss is
$$
\ell = \frac{1}{n}\sum_{i=1}^{n}(o^{(i)} - y^{(i)})^2.
$$

Using backpropagation and the fact that $\sigma'(u) = \sigma(u)(1 - \sigma(u))$, we have:
$$
\frac{\partial \ell}{\partial w^{[1]}_{1,2}}
= \frac{2}{n}\sum_{i=1}^{n} (o^{(i)} - y^{(i)})
\, o^{(i)}(1 - o^{(i)}) \, w^{[2]}_2 \, h^{(i)}_2(1 - h^{(i)}_2)\, x^{(i)}_1.
$$

The gradient descent update (with learning rate $\alpha$) is therefore:
$$
\boxed{
w^{[1]}_{1,2} \leftarrow
w^{[1]}_{1,2}
-
\alpha
\cdot
\frac{2}{n}\sum_{i=1}^{n} (o^{(i)} - y^{(i)})
\, o^{(i)}(1 - o^{(i)}) \, w^{[2]}_2 \, h^{(i)}_2(1 - h^{(i)}_2)\, x^{(i)}_1
}.
$$

		
\end{answer}
