\begin{answer}

For a single example $x_i, y_i$

\begin{align*}
    \exp(-f(x_i)y_i) 
    &= \exp(-\sum_{t=1}^{T}\tilde{w}_t f_t(x_{i})y_i) \\
    &= \exp(-\tilde{w}_1 f_1(x_{i})y_i) \cdot \exp(-\tilde{w}_2 f_2(x_{i})y_i) \dots \exp(-\tilde{w}_T f_T(x_{i})y_i) \\
    &= \prod_{t=1}^{T}\exp(-\tilde{w}_t f_t(x_{i})y_i)
\end{align*}

For the whole dataset
$$
\frac{1}{n} \sum_{i=1}^{n} \exp(-f(x_i)y_i) = \frac{1}{n} \sum_{i=1}^{n} \prod_{t=1}^{T}\exp(-\tilde{w}_t f_t(x_{i})y_i)
$$

Since $\alpha_{i,1}=\frac{1}{n}$, then
$$
\frac{1}{n} \sum_{i=1}^{n} \exp(-f(x_i)y_i) = \sum_{i=1}^{n} \alpha_{i,1} \prod_{t=1}^{T}\exp(-\tilde{w}_t f_t(x_{i})y_i)
$$

For $t=1$:
$$
 \sum_{i=1}^{n} \alpha_{i,1} \exp(-\tilde{w}_1 f_1(x_{i})y_i) \prod_{t=1}^{T}\exp(-\tilde{w}_t f_t(x_{i})y_i) = Z_1 \sum_{i=1}^{n} \underbrace{\frac{\alpha_{i,1} \exp(-\tilde{w}_1 f_1(x_{i})y_i)}{Z_{1}}}_{\alpha_{i,2}} \prod_{t=2}^{T}\exp(-\tilde{w}_t f_t(x_{i})y_i)
$$

For $t=2$:
$$
= Z_1 Z_2 \sum_{i=1}^{n} \underbrace{\frac{\alpha_{i,2} \exp(-\tilde{w}_2 f_2(x_{i})y_i)}{Z_{2}}}_{\alpha_i,3} \prod_{t=3}^{T}\exp(-\tilde{w}_t f_t(x_{i})y_i)
$$

For $t=3, \dots, T$, and considering $\sum_{i=1}^{n} \alpha_{i, t} = 1$
$$
= \prod_{t=1}^{T} Z_t \sum_{i=1}^{n} \alpha_{i,t+1} = \prod_{t=1}^{T} Z_t
$$

Finally,
$$
\boxed{
\frac{1}{n} \sum_{i=1}^{n} \exp(-f(x_i)y_i) = \prod_{t=1}^{T} Z_t
}
$$

\end{answer}